Revised the sequential semantics to deal with incomplete transactions

src/SemSeq.v
@@ -2,19 +2,31 @@ Require Import Bool List String Peano_dec.
 Require Import Permutation.
 Require Import Common FMap Syntax Semantics.
 
-Definition NoInternalsQ (sys: System) (q: Queue) :=
-  Forall (fun m => isInternal sys (msgFrom (msg_id m)) = false) q.
+Record AtomicMsg :=
+  { atm_msg : Msg;
+    atm_active : bool
+  }.
 
-Definition NoInternalsC (sys: System) (c: Channels) :=
-  forall cidx, c@[cidx] >>=[True] (fun q => NoInternalsQ sys q).
+Instance AtomicMsg_HasMsg : HasMsg AtomicMsg :=
+  { getMsg := atm_msg }.
 
-Definition NoInternalsMF (sys: System) (mf: MsgsFrom) :=
-  forall fr, mf@[fr] >>=[True] (fun c => NoInternalsC sys c).
+Definition toAtomicMsgs (active: bool) (msgs: list Msg) :=
+  map (fun m => {| atm_msg := m; atm_active := active |}) msgs.
+Definition toAtomicMsgsT := toAtomicMsgs true.
+Definition toAtomicMsgsF := toAtomicMsgs false.
 
-Definition NoInternalsM (sys: System) (msgs: Messages) :=
-  forall to, msgs@[to] >>=[True] (fun mf => NoInternalsMF sys mf).
+Section Deactivation.
 
-Inductive step_seq (sys: System) : State -> Label -> State -> Prop :=
+  Definition deactivate (am: AtomicMsg) :=
+    {| atm_msg := atm_msg am; atm_active := false |}.
+  Definition deactivateQ (q: Queue AtomicMsg) := map deactivate q.
+  Definition deactivateC (cs: Channels AtomicMsg) := M.map deactivateQ cs.
+  Definition deactivateMF (mf: MsgsFrom AtomicMsg) := M.map deactivateC mf.
+  Definition deactivateM (msgs: Messages AtomicMsg) := M.map deactivateMF msgs.
+
+End Deactivation.
+
+Inductive step_seq (sys: System) : State AtomicMsg -> Label -> State AtomicMsg -> Prop :=
 | SsSlt: forall s, step_seq sys s emptyLabel s
 | SsInt: forall oss oims obj idx mf os pos fmsg fpmsg fidx fchn outs,
     In obj (sys_objs sys) ->
@@ -22,29 +34,27 @@ Inductive step_seq (sys: System) : State -> Label -> State -> Prop :=
     oss@[idx] = Some os ->
     oims@[idx] = Some mf ->
 
+    (atm_active fmsg = true \/ isExternal sys fidx = true) ->
+    
     firstMF fidx fchn mf = Some fmsg ->
-    msg_id fmsg = pmsg_mid fpmsg ->
-    ValidMsgId fidx idx fchn fmsg ->
+    msg_id (getMsg fmsg) = pmsg_mid fpmsg ->
+    ValidMsgId fidx idx fchn (getMsg fmsg) ->
     In fpmsg (obj_trs obj) ->
     pmsg_precond fpmsg os ->
-    pmsg_postcond fpmsg os (msg_value fmsg) pos ->
-    outs = pmsg_outs fpmsg os (msg_value fmsg) ->
-
-    (* This is the only one additional condition compared with [step_mod];
-     * The system starts handling external messages only when there are no internal
-     * messages.
-     *)
-    (isExternal sys fidx = true -> NoInternalsM sys oims) ->
-
+    pmsg_postcond fpmsg os (msg_value (getMsg fmsg)) pos ->
+    outs = pmsg_outs fpmsg os (msg_value (getMsg fmsg)) ->
     step_seq sys {| st_oss := oss; st_msgs := oims |}
-             (buildLabel nil (Some fmsg) (extOuts sys outs))
+             (buildLabel nil (Some (getMsg fmsg)) (extOuts sys outs))
              {| st_oss := oss +[ idx <- pos ];
-                st_msgs := distributeMsgs (intOuts sys outs) oims |}
+                st_msgs := distributeMsgs (toAtomicMsgsT (intOuts sys outs))
+                                          (if isExternal sys fidx
+                                           then deactivateM oims
+                                           else oims) |}
 | SsExt: forall from emsgs oss oims,
-    ~ In from (indicesOf sys) ->
+    isExternal sys from = true ->
     emsgs <> nil ->
-    SubList (map (fun m => msgTo (msg_id m)) emsgs) (indicesOf sys) ->
+    SubList (map (fun m => mid_to (msg_id m)) emsgs) (indicesOf sys) ->
     step_seq sys {| st_oss := oss; st_msgs := oims |}
              (buildLabel emsgs None nil)
-             {| st_oss := oss; st_msgs := distributeMsgs emsgs oims |}.
+             {| st_oss := oss; st_msgs := distributeMsgs (toAtomicMsgsF emsgs) oims |}.
 
