src/Semantics.v
@@ -1,16 +1,26 @@
 Require Import Bool List String Peano_dec.
 Require Import Common FMap Syntax.
 
-Section Messages.
+Set Implicit Arguments.
 
-  Definition Queue := list Msg.
+Class HasMsg (MsgT: Type) :=
+  { getMsg : MsgT -> Msg }.
+
+Instance Msg_HasMsg : HasMsg Msg :=
+  { getMsg := id }.
+
+Section Messages.
+  Variable (MsgT: Type).
+  Context `{HasMsg MsgT}.
+
+  Definition Queue := list MsgT.
   Definition Channels := M.t (* channel index *) Queue.
   Definition MsgsFrom := M.t (* from *) Channels.
   Definition Messages := M.t (* to *) MsgsFrom.
 
   Definition firstQ (q: Queue) := hd_error q.
   Definition deq (q: Queue): Queue := tl q.
-  Definition enq (m: Msg) (q: Queue): Queue := q ++ (m :: nil).
+  Definition enq (m: MsgT) (q: Queue): Queue := q ++ (m :: nil).
   Definition EmptyQ (q: Queue) := q = nil.
 
   Definition findC (chn: IdxT) (cs: Channels): Queue :=
@@ -22,7 +32,7 @@ Section Messages.
     | Some q => cs +[chn <- deq q]
     | None => cs
     end.
-  Definition enqC (chn: IdxT) (m: Msg) (cs: Channels): Channels :=
+  Definition enqC (chn: IdxT) (m: MsgT) (cs: Channels): Channels :=
     match cs@[chn] with
     | Some q => cs +[chn <- enq m q]
     | None => cs +[chn <- enq m nil]
@@ -47,7 +57,7 @@ Section Messages.
     | Some cs => mf +[from <- deqC chn cs]
     | None => mf
     end.
-  Definition enqMF (from chn: IdxT) (m: Msg) (mf: MsgsFrom): MsgsFrom :=
+  Definition enqMF (from chn: IdxT) (m: MsgT) (mf: MsgsFrom): MsgsFrom :=
     match mf@[from] with
     | Some cs => mf +[from <- enqC chn m cs]
     | None => mf +[from <- enqC chn m (M.empty _)]
@@ -73,7 +83,7 @@ Section Messages.
     | Some froms => msgs +[to <- deqMF from chn froms]
     | None => msgs
     end.
-  Definition enqM (from to chn: IdxT) (m: Msg) (msgs: Messages): Messages :=
+  Definition enqM (from to chn: IdxT) (m: MsgT) (msgs: Messages): Messages :=
     match msgs@[to] with
     | Some froms => msgs +[to <- enqMF from chn m froms]
     | None => msgs +[to <- enqMF from chn m (M.empty _)]
@@ -90,6 +100,18 @@ Section Messages.
     eexists; split; auto.
   Qed.
 
+  Definition distributeMsg (msg: MsgT) (msgs: Messages): Messages :=
+    enqM (mid_from (msg_id (getMsg msg)))
+         (mid_to (msg_id (getMsg msg)))
+         (mid_chn (msg_id (getMsg msg))) msg msgs.
+
+  Fixpoint distributeMsgs (nmsgs: list MsgT) (msgs: Messages): Messages :=
+    match nmsgs with
+    | nil => msgs
+    | msg :: nmsgs' =>
+      distributeMsgs nmsgs' (distributeMsg msg msgs)
+    end.
+  
 End Messages.
 
 Section Semantics.
@@ -114,8 +136,8 @@ Section Semantics.
   Definition ObjectStates := M.t StateT.
 
   Definition ValidMsgId (from to chn: IdxT) (msg: Msg) :=
-    msgFrom (msg_id msg) = from /\
-    msgTo (msg_id msg) = to /\
+    mid_from (msg_id msg) = from /\
+    mid_to (msg_id msg) = to /\
     mid_chn (msg_id msg) = chn.
 
   (* A set of messages are "valid outputs" if
@@ -125,8 +147,8 @@ Section Semantics.
    * TODO: syntax has to ensure [ValidOuts], or by well-formedness.
    *)
   Definition ValidOuts (idx: IdxT) (msgs: list Msg) :=
-    Forall (fun m => msgFrom (msg_id m) = idx /\ msgTo (msg_id m) <> idx) msgs /\
-    NoDup (map (fun m => (msgTo (msg_id m), mid_chn (msg_id m))) msgs).
+    Forall (fun m => mid_from (msg_id m) = idx /\ mid_to (msg_id m) <> idx) msgs /\
+    NoDup (map (fun m => (mid_to (msg_id m), mid_chn (msg_id m))) msgs).
 
   (* [step_obj] is for a step by a single object that either handles an 
    * internal message, or receives an external message.
@@ -137,8 +159,8 @@ Section Semantics.
    * For an external message: it just receives the message and add it to a 
    * proper queue.
    *)
-  Inductive step_obj (obj: Object): StateT -> MsgsFrom -> Label ->
-                                    StateT -> MsgsFrom -> Prop :=
+  Inductive step_obj (obj: Object): StateT -> MsgsFrom Msg -> Label ->
+                                    StateT -> MsgsFrom Msg -> Prop :=
   | SoSlt: forall os mf, step_obj obj os mf emptyLabel os mf
   | SoInt: forall os mf fidx fchn fmsg fpmsg pos,
       firstMF fidx fchn mf = Some fmsg ->
@@ -152,21 +174,24 @@ Section Semantics.
                (buildLabel nil (Some fmsg) (pmsg_outs fpmsg os (msg_value fmsg)))
                pos (deqMF fidx fchn mf)
   | SoExt: forall os mf emsg,
-      msgTo (msg_id emsg) = obj_idx obj ->
-      msgFrom (msg_id emsg) <> obj_idx obj ->
+      mid_to (msg_id emsg) = obj_idx obj ->
+      mid_from (msg_id emsg) <> obj_idx obj ->
       step_obj obj os mf
                (buildLabel (o2l (Some emsg)) None nil)
-               os (enqMF (msgFrom (msg_id emsg))
+               os (enqMF (mid_from (msg_id emsg))
                          (mid_chn (msg_id emsg))
                          emsg mf).
 
-  Record State := { st_oss: ObjectStates; st_msgs: Messages }.
+  Record State MsgT :=
+    { st_oss: ObjectStates;
+      st_msgs: Messages MsgT
+    }.
 
-  Definition DisjointState (st1 st2: State) :=
+  Definition DisjointState {MsgT} (st1 st2: State MsgT) :=
     M.Disj (st_oss st1) (st_oss st2) /\
     M.Disj (st_msgs st1) (st_msgs st2).
 
-  Definition combineState (st1 st2: State) :=
+  Definition combineState {MsgT} (st1 st2: State MsgT) :=
     {| st_oss := M.union (st_oss st1) (st_oss st2);
        st_msgs := M.union (st_msgs st1) (st_msgs st2) |}.
   Infix "+s" := combineState (at level 30).
@@ -184,7 +209,7 @@ Section Semantics.
 
   (* Definition ValidLabel (l: Label) := *)
   (*   match lbl_hdl l with *)
-  (*   | Some hmsg => lbl_ins l = nil /\ ValidOuts (msgTo (msg_id hmsg)) (lbl_outs l) *)
+  (*   | Some hmsg => lbl_ins l = nil /\ ValidOuts (mid_to (msg_id hmsg)) (lbl_outs l) *)
   (*   | None => lbl_outs l = nil /\ exists from, ValidOuts from (lbl_ins l) *)
   (*   end. *)
 
@@ -206,7 +231,7 @@ Section Semantics.
   (* [step_sys] either lifts a step by [step_obj] to a given system, or
    * combines two steps.
    *)
-  Inductive step_sys (sys: System) : State -> Label -> State -> Prop :=
+  Inductive step_sys (sys: System) : State Msg -> Label -> State Msg -> Prop :=
   | SsLift: forall oss idx (obj: Object) (os: StateT)
                    oims mf lbl pos pmf,
       In obj (sys_objs sys) ->
@@ -232,35 +257,27 @@ Section Semantics.
 
   Definition Hidden (sys: System) (l: Label) :=
     match lbl_hdl l with
-    | Some _ => Forall (fun m => isExternal sys (msgTo (msg_id m)) = true) (lbl_outs l)
-    | _ => Forall (fun m => isExternal sys (msgFrom (msg_id m)) = true) (lbl_ins l)
+    | Some _ => Forall (fun m => isExternal sys (mid_to (msg_id m)) = true) (lbl_outs l)
+    | _ => Forall (fun m => isExternal sys (mid_from (msg_id m)) = true) (lbl_ins l)
     end.
 
-  Inductive step_mod : System -> State -> Label -> State -> Prop :=
+  Inductive step_mod : System -> State Msg -> Label -> State Msg -> Prop :=
   | StepMod:
       forall sys st1 l st2,
         step_sys sys st1 l st2 ->
         Hidden sys l ->
         step_mod sys st1 l st2.
 
-  Definition distributeMsg (msg: Msg) (msgs: Messages): Messages :=
-    enqM (msgFrom (msg_id msg)) (msgTo (msg_id msg)) (mid_chn (msg_id msg)) msg msgs.
-  
-  Fixpoint distributeMsgs (nmsgs: list Msg) (msgs: Messages): Messages :=
-    match nmsgs with
-    | nil => msgs
-    | msg :: nmsgs' =>
-      distributeMsgs nmsgs' (distributeMsg msg msgs)
-    end.
-  
   Definition intOuts (sys: System) (outs: list Msg) :=
-    filter (fun m => isInternal sys (msgTo (msg_id m))) outs.
+    filter (fun m => isInternal sys (mid_to (msg_id m))) outs.
   Definition extOuts (sys: System) (outs: list Msg) :=
-    filter (fun m => isExternal sys (msgTo (msg_id m))) outs.
+    filter (fun m => isExternal sys (mid_to (msg_id m))) outs.
 
+  Definition Step MsgT := System -> State MsgT -> Label -> State MsgT -> Prop.
+  
   (* NOTE: the head is the youngest *)
-  Inductive steps (step: System -> State -> Label -> State -> Prop)
-            (sys: System) : State -> list Label -> State -> Prop :=
+  Inductive steps {MsgT} (step: Step MsgT)
+            (sys: System) : State MsgT -> list Label -> State MsgT -> Prop :=
   | StepsNil: forall st, steps step sys st nil st
   | StepsCons:
       forall st1 ll st2,
@@ -277,7 +294,7 @@ Section Semantics.
     | obj :: sys' => (getObjectStatesInit sys') +[obj_idx obj <- obj_state_init obj]
     end.
 
-  Definition getStateInit (sys: System) :=
+  Definition getStateInit {MsgT} (sys: System): State MsgT :=
     {| st_oss := getObjectStatesInit (sys_objs sys);
        st_msgs := [] |}.
 
@@ -326,16 +343,16 @@ Section Semantics.
     | l :: tr' => (toBLabel l) ::> (behaviorOf tr')
     end.
 
-  Inductive Behavior (step: System -> State -> Label -> State -> Prop)
-    : System -> Trace -> Prop :=
+  Inductive Behavior {MsgT} (step: Step MsgT) : System -> Trace -> Prop :=
   | Behv: forall sys ll st,
       steps step sys (getStateInit sys) ll st ->
       forall tr,
         tr = behaviorOf ll ->
         Behavior step sys tr.
 
-  Definition Refines (stepI stepS: System -> State -> Label -> State -> Prop)
-             (p: BLabel -> BLabel) (impl spec: System) :=
+  Definition Refines {MsgI MsgS} (stepI: Step MsgI) (stepS: Step MsgS)
+             (p: BLabel -> BLabel)
+             (impl spec: System) :=
     forall ll, Behavior stepI impl ll ->
                Behavior stepS spec (map p ll).
 
