src/Syntax.v
@@ -11,34 +11,18 @@ Section Msg.
 
   Definition IdxT := nat.
 
-  Definition MsgT := string.
-  Definition msgT_dec := string_dec.
-
-  (* A message is always either a request or a response. *)
-  Inductive RqRs := Rq | Rs.
-
   Record MsgId :=
-    { mid_rq : IdxT; (* an object that requests this message *)
-      mid_rs : IdxT; (* an object that responses this message *)
-      mid_type : MsgT;
-      mid_rqrs : RqRs;
+    { mid_type : IdxT;
+      mid_from : IdxT; (* an object that requests this message *)
+      mid_to : IdxT; (* an object that responses this message *)
       mid_chn : IdxT (* which channel (queue) to use *)
     }.
 
-  Definition buildMsgId rq rs ty rr cn :=
-    {| mid_rq := rq; mid_rs := rs; mid_type := ty; mid_rqrs := rr; mid_chn := cn |}.
+  Definition buildMsgId ty fr to cn :=
+    {| mid_type := ty; mid_from := fr; mid_to := to; mid_chn := cn |}.
 
   Definition msgId_dec: forall m1 m2: MsgId, {m1 = m2} + {m1 <> m2}.
   Proof. repeat decide equality. Defined.
-
-  Definition isTrsPair (rq rs: MsgId) :=
-    (if mid_rq rq ==n mid_rq rs then true else false)
-      && (if mid_rs rq ==n mid_rs rs then true else false)
-      && (if msgT_dec (mid_type rq) (mid_type rs) then true else false)
-      && (match mid_rqrs rq, mid_rqrs rs with
-          | Rq, Rs => true
-          | _, _ => false
-          end).
 
   Inductive Value :=
   | VUnit
@@ -56,18 +40,6 @@ Section Msg.
 
   Definition msg_dec: forall m1 m2: Msg, {m1 = m2} + {m1 <> m2}.
   Proof. repeat decide equality. Defined.
-
-  Definition msgFrom (msg: MsgId) :=
-    match mid_rqrs msg with
-    | Rq => mid_rq msg
-    | Rs => mid_rs msg
-    end.
-
-  Definition msgTo (msg: MsgId) :=
-    match mid_rqrs msg with
-    | Rq => mid_rs msg
-    | Rs => mid_rq msg
-    end.
 
 End Msg.
 
