src/SemFacts.v
@@ -2,7 +2,7 @@ Require Import Bool List String Peano_dec.
 Require Import Common FMap Syntax Semantics.
 
 Theorem refines_refl:
-  forall step sys, step # step |-- sys ⊑[id] sys.
+  forall (step: Step Msg) sys, step # step |-- sys ⊑[id] sys.
 Proof.
   unfold Refines; intros.
   rewrite map_id.
@@ -10,7 +10,7 @@ Proof.
 Qed.
 
 Theorem refines_trans:
-  forall step1 step2 step3 s1 s2 s3 p q,
+  forall (step1 step2 step3: Step Msg) s1 s2 s3 p q,
     step1 # step2 |-- s1 ⊑[p] s2 ->
     step2 # step3 |-- s2 ⊑[q] s3 ->
     step1 # step3 |-- s1 ⊑[fun l => q (p l)] s3.
