src/SerialFacts.v
@@ -16,21 +16,16 @@ Lemma equiv_history_behavior:
 Proof.
 Admitted.
 
-Lemma sequential_steps:
-  forall sys ll st,
-    Sequential sys (historyOf ll) ->
-    steps step_mod sys (getStateInit sys) ll st ->
-    steps step_seq sys (getStateInit sys) ll st.
-Proof.
-  unfold Sequential; intros.
-  destruct H as [trs [? ?]].
+(* Lemma sequential_steps: *)
+(*   forall sys ll st, *)
+(*     Sequential sys (historyOf ll) -> *)
+(*     steps step_mod sys (getStateInit sys) ll st -> *)
+(*     steps step_seq sys (getStateInit sys) ll st. *)
+(* Proof. *)
+(*   unfold Sequential; intros. *)
+(*   destruct H as [trs [? ?]]. *)
 
-  (* This is currently WRONG since the requirement of sequential
-   * semantics (no internal messages to allow an external request)
-   * does not work for any [IncompleteTrs] transactions.
-   *)
-  
-Admitted.
+(* Admitted. *)
 
 Theorem serializable_step_seq:
   forall sys ll st,
@@ -38,17 +33,17 @@ Theorem serializable_step_seq:
     Serializable sys step_mod ll ->
     Behavior step_seq sys (behaviorOf ll).
 Proof.
-  unfold Serializable; intros.
-  destruct H0 as [sll [sst [? [? ?]]]].
+  (* unfold Serializable; intros. *)
+  (* destruct H0 as [sll [sst [? [? ?]]]]. *)
 
-  pose proof (equiv_history_behavior H H0 H2) as Hnll.
-  destruct Hnll as [nll [? [? ?]]].
+  (* pose proof (equiv_history_behavior H H0 H2) as Hnll. *)
+  (* destruct Hnll as [nll [? [? ?]]]. *)
 
-  eapply Behv with (st:= sst) (ll:= nll); eauto.
+  (* eapply Behv with (st:= sst) (ll:= nll); eauto. *)
 
-  rewrite <-H4 in H1.
-  auto using sequential_steps.
-Qed.
+  (* rewrite <-H4 in H1. *)
+  (* auto using sequential_steps. *)
+Admitted.
 
 Theorem sequential_step_seq:
   forall sys,
